One proof of process

Palphabeta.v
@@ -45,6 +45,7 @@ Hypothesis wNw : ~~ cwin w.
 Hypothesis wNb : ~~ cwin b.
 Hypothesis wbWf : wf_state (w lor b).
 Hypothesis wbL : w land b = 0.
+Hypothesis wbH : has_move (w lor b).
 
 Lemma ufixE v : ufix v land 1 = 1.
 Proof.
@@ -76,6 +77,114 @@ Definition valid_list (l : seq (int * int)) := forall m : int * int,
     m \in l -> 
     exists i j : nat, cmove (w lor b) i j /\
     m.1 = lsl 1 (of_nat i * horizontal + of_nat j).
+
+
+Definition get_max (ms : seq (int * int)) := 
+  maxn LOSS 
+    (\max_(i < nwidth) \max_(j < nheight | cmove (w lor b) i j && 
+            (lsl 1 (of_nat i * horizontal + of_nat j) \notin map fst ms))
+           wcomp (eval b (mk_move w i j))).
+
+Lemma get_max_range ms : 
+  [\/ get_max ms = LOSS, get_max ms = DRAW | get_max ms = WIN].
+Proof.
+rewrite /get_max; set u := \max_(_ < _) _.
+suff : [\/ u = 0%N, u = LOSS, u = DRAW | u = WIN].
+  by case=> ->; (try by apply: Or31); (try by apply: Or32); apply: Or33.
+rewrite /u; elim: {-2}nwidth (leqnn nwidth) => [|n IH nLw].
+  by rewrite big_ord0 => _; apply: Or41.
+rewrite big_ord_recr /=.
+set v := \max_(j < nheight | _) _.
+suff : [\/ v = 0%N, v = LOSS, v = DRAW | v = WIN].
+  by case => ->; case: (IH (ltnW nLw)) => ->;
+       (try by apply: Or41); (try by apply: Or42); (try by apply: Or43); 
+      apply: Or44.
+rewrite /v big_mkcond /=.
+elim: {-2}nheight (leqnn nheight) => [|m IH1 mLh].
+  by rewrite big_ord0 => _; apply: Or41.
+rewrite big_ord_recr /=.
+by case/or3P: (evalOr b (mk_move w n m)) => /eqP->; case: ifP => _; case: (IH1 (ltnW mLh)) => ->;
+       (try by apply: Or41); (try by apply: Or42); (try by apply: Or43); 
+      apply: Or44.
+Qed.
+
+Lemma get_max_nil : get_max [::] = eval w b.
+Proof.
+rewrite evalS (negPf wNw) /= wbH /get_max.
+case/existsP : wbH => /= i /existsP [/= j ijM].
+rewrite (bigD1 i) //= maxnA [in RHS](bigD1 i) //=; congr maxn.
+  rewrite (bigD1 j) ?andbT //= maxnA [in RHS](bigD1 j) //=; congr maxn.
+    by case/or3P: (evalOr b (mk_move w i j)) => /eqP->.
+  by apply: eq_bigl => k; rewrite andbT.
+by apply: eq_bigr => i1 _; apply: eq_bigl => j1; rewrite andbT.
+Qed.
+
+Lemma get_max_cons m i j ms :
+  uniq (map fst (m :: ms)) ->
+  m.1 = (lsl one (of_nat i * horizontal + of_nat j)) -> cmove (w lor b) i j -> 
+  get_max ms = maxn (wcomp (eval b (mk_move w i j))) (get_max (m :: ms)).
+Proof.
+move=> msU mmE ijM. 
+have iLw : i < nwidth by case/and3P: ijM.
+have jLh : j < nheight by case/and3P: ijM.
+rewrite /get_max.
+rewrite (bigD1 (Ordinal iLw)) //= [in RHS](bigD1 (Ordinal iLw)) //= !maxnA; congr maxn.
+  rewrite (bigD1 (Ordinal jLh)) //=; last first.
+    by rewrite ijM; move: msU => /= /andP[]; rewrite mmE => ->.
+  rewrite maxnA; congr maxn; first by rewrite maxnC.
+  apply: eq_bigl => k /=; rewrite -andbA; congr (_ && _).
+  rewrite inE negb_or andbC mmE; congr (_ && _).
+  (apply/idP/idP => /=; 
+  move=> /eqP HH1; apply/eqP; contradict HH1); last first.
+    by move/val_eqP : HH1 => /= /eqP->.
+  apply/val_eqP/eqP => /=.
+  move/(congr1 (fun x => to_nat x)) : HH1 => /eqP HH2.
+  have kLhe : k < nhorizontal by apply: ltn_trans (ltn_ord _) _.
+  have jLhe : j < nhorizontal by apply: ltn_trans jLh _.
+  rewrite [X in X == _]to_nat_lsl_one ihjE // in HH2; last by apply: ihjLd.
+  rewrite [X in _ == X]to_nat_lsl_one ihjE // in HH2; last by apply: ihjLd.
+  rewrite eqn_exp2l // eqn_add2l in HH2 .
+  by apply/eqP.
+apply: eq_bigr => i1 /eqP /val_eqP /= i1Di.
+apply: eq_bigl => j1; congr (_ && _); rewrite inE negb_or.
+rewrite -{1}[LHS]andbT [RHS]andbC.
+congr (_ && _); apply/sym_equal/idP.
+rewrite mmE; move/eqP: i1Di => i1Di; apply/eqP; contradict i1Di.
+move/(congr1 (fun x => to_nat x)) : i1Di => /eqP HH2.
+have j1Lhe : j1 < nhorizontal by apply: ltn_trans (ltn_ord _) _.
+have jLhe : j < nhorizontal by apply: ltn_trans jLh _.
+rewrite [X in X == _]to_nat_lsl_one ihjE // in HH2; last by apply: ihjLd.
+rewrite [X in _ == X]to_nat_lsl_one ihjE // in HH2; last by apply: ihjLd.
+rewrite eqn_exp2l // in HH2.
+case: (ltngtP i1 i) => // [i1Li | iLi1].
+  suff : i1 * nhorizontal + j1 < i * nhorizontal + j by rewrite (eqP HH2) ltnn.
+  apply: leq_trans (_ : i1.+1  * nhorizontal <= _).
+    by rewrite mulSn addnC ltn_add2r.
+  by apply: leq_trans (leq_addr _ _); rewrite leq_mul2r.
+suff : i * nhorizontal + j < i1 * nhorizontal + j1 by rewrite (eqP HH2) ltnn.
+apply: leq_trans (_ : i.+1  * nhorizontal <= _).
+  by rewrite mulSn addnC ltn_add2r.
+by apply: leq_trans (leq_addr _ _); rewrite leq_mul2r.
+Qed.
+
+
+Definition valid_sc (ms : seq (int * int)) sc := 
+  down_score sc <= get_max ms <= up_score sc. 
+
+Lemma valid_sc_range ms sc :
+  valid_sc ms sc -> 
+   [\/ sc = loss, sc = draw | sc = win] \/
+   [\/ sc = unknown, sc = lossdraw | sc = drawwin].
+Proof.
+rewrite /valid_sc => /andP[] /leq_trans H /(H _).
+rewrite /down_score /up_score.
+case: eqP => [->//|_]; first by right; apply: Or31.
+case: eqP => [->//|_]; first by left; apply: Or31.
+case: eqP => [->//|_]; first by right; apply: Or32.
+case: eqP => [->//|_]; first by left; apply: Or32.
+case: eqP => [->//|_]; first by right; apply: Or33.
+by case: eqP => [->//|]; first by left; apply: Or33.
+Qed.
 
 Lemma valid_cons m (l : seq (int * int)) :
    valid_list (m :: l) -> 
@@ -120,23 +229,65 @@ Proof. by have /or3P[] := evalOr w1 b1 => /eqP->. Qed.
 Lemma leq_loss_eval w1 b1 : LOSS <= eval w1 b1.
 Proof. by have /or3P[] := evalOr w1 b1 => /eqP->. Qed.
 
-Lemma process_correct  ms alpha sc sc1 v v1 h h1:
-  valid_list ms -> valid_hash_table h -> valid_ab alpha beta ->
+Lemma leq_down_score (a1 c1 : int) (b1 d1 : nat) :
+  [\/ b1 = LOSS, b1 = DRAW | b1 = WIN] ->
+  [\/ d1 =  LOSS, d1 = DRAW | d1 = WIN] ->
+  [\/ a1 =  loss, a1 = draw | a1 = win] \/
+  [\/  a1 = lossdraw | a1 = drawwin]  ->
+  [\/ c1 =  loss, c1 = draw | c1 = win] \/
+  [\/ c1 = lossdraw | c1 = drawwin]  ->
+  down_score a1 <= b1 <= up_score a1 ->
+  down_score c1 <= d1 <= up_score c1 ->
+  to_nat a1 <= to_nat c1 ->
+  down_score c1 <= maxn b1 d1 <= up_score c1.
+Proof.
+case => ->; case => -> //; case; case => -> //; case; case => -> //.
+Qed.
+
+Lemma ltn_down_score (a1 c1 : int) (b1 d1 : nat) :
+  [\/ b1 = LOSS, b1 = DRAW | b1 = WIN] ->
+  [\/ d1 =  LOSS, d1 = DRAW | d1 = WIN] ->
+  [\/ a1 =  loss, a1 = draw | a1 = win] \/
+  [\/  a1 = lossdraw | a1 = drawwin]  ->
+  [\/ c1 =  loss, c1 = draw | c1 = win] \/
+  [\/ c1 = lossdraw | c1 = drawwin]  ->
+  down_score a1 <= b1 <= up_score a1 ->
+  down_score c1 <= d1 <= up_score c1 ->
+  to_nat c1 < to_nat a1 ->
+  down_score a1 <= maxn b1 d1 <= up_score a1.
+Proof.
+case => ->; case => -> //; case; case => -> //; case; case => -> //.
+Qed.
+
+Lemma process_correct ms alpha sc sc1 v v1 h h1 :
+  sc != unknown ->
+  uniq (map fst ms) -> valid_list ms -> valid_sc ms sc ->
+  valid_hash_table h -> valid_ab alpha beta ->
   process ms alpha sc v h =  PRes sc1 v1 h1 ->
-  valid_hash_table h1.
+  valid_eval w b sc1 /\ valid_hash_table h1.
 Proof.
 elim: ms alpha sc sc1 v v1 h h1 =>
-   [|[m x] ms IH] alpha sc sc1 v v1 h h1 Vms Vh Vab /=.
+   [|[m x] ms IH] alpha sc sc1 v v1 h h1 scDu Ums Vms Vsc Vh Vab /=.
   case: neqbP.
     move=> HH.
     suff eD : DRAW <= eval w b <= DRAW.
-      by case => dE _ <-; apply: valid_has_table_valid_hput.
-    admit.
+      case => dE _ <-; split; first by rewrite -dE.
+      by apply: valid_has_table_valid_hput.
+    have hsE : (hs = lossdraw) \/ (hs = drawwin).
+      have := HH; have := hs_range => [] [] -> //;  (try by left); (try by right).
+      by have /valid_sc_range := Vsc; case; case => ->.
+    case: hsE => hsE.
+      apply/andP; split; last by case/andP : hsV; rewrite hsE.
+      have scE : sc = drawwin by apply/to_nat_inj; rewrite HH hsE.
+      by have := Vsc; rewrite /valid_sc get_max_nil scE; case/andP.
+    have scE : sc = lossdraw by apply/to_nat_inj; rewrite HH hsE.
+    apply/andP; split; first by case/andP : hsV; rewrite hsE.
+    by have := Vsc; rewrite /valid_sc get_max_nil scE; case/andP.
   move=> HH.
   suff eD : down_score sc <= eval w b <= up_score sc.
-    case => dE _ <-.
+    case => dE _ <-; split; first by rewrite -dE.
     by apply: valid_has_table_valid_hput.
-  admit.
+  by have := Vsc; rewrite /valid_sc get_max_nil.
 case E : ab => [s2 v2 h2].
 case: (ab_correct _ _ _ _ _ _ _ _ _ _ _ E) => // [|s2Nu h2V vEs2].
   by apply: valid_ab_rev.
@@ -147,10 +298,62 @@ have us2Le : wcomp (up_score s2) <= eval w b.
   have /(leq_trans _)-> // := leq_eval_move _ _ ijM.
   by apply: leq_wcomp; rewrite -mmE; case/andP: vEs2.
 case: nltbP => [rs2Lb|/negP].
-  case: nlebP => _; first by apply: IH.
-  case: nlebP => [_|/negP]; first by apply: IH.
+  case: nlebP => [HH|/negP].
+    apply: IH => //; first by case/andP:  Ums.
+    rewrite /valid_sc (@get_max_cons (m, x) i j) //.
+    apply: leq_down_score HH => //.
+    - by have := evalOr b (mk_move w i j); case/or3P => /eqP->;
+        try (by apply: Or31); try (by apply: Or32); apply: Or33.
+    - by apply: get_max_range.
+    - by move: s2Nu; move/valid_evalE: vEs2; case; case=> -> //;
+      try(by left; (try by apply: Or31);(try by apply: Or32); apply: Or33);
+        right; (try by left); right.
+    - by move: scDu; move/valid_sc_range: Vsc; case; case=> -> //;
+      try(by left; (try by apply: Or31);(try by apply: Or32); apply: Or33);
+        right; (try by left); right.
+    have := s2Nu; have := vEs2.
+    by rewrite /valid_eval; move/valid_evalE : vEs2; rewrite mmE;
+          case; case=> ->;
+          case /or3P: (evalOr b (mk_move w i j)) => /eqP->.
+  rewrite -ltnNge=> scLrs2.
+  case: nlebP => [Hd|/negP].
+    apply: IH => //.
+    - by move/valid_evalE : vEs2; case; case => ->.
+    - by case/andP: Ums.
+    rewrite /valid_sc (@get_max_cons (m, x) i j) //. 
+    apply: ltn_down_score scLrs2 => //.
+    - by have := evalOr b (mk_move w i j); case/or3P => /eqP->;
+        try (by apply: Or31); try (by apply: Or32); apply: Or33.
+    - by apply: get_max_range.
+    - by move: s2Nu; move/valid_evalE: vEs2; case; case=> -> //;
+      try(by left; (try by apply: Or31);(try by apply: Or32); apply: Or33);
+        right; (try by left); right.
+    - by move: scDu; move/valid_sc_range: Vsc; case; case=> -> //;
+      try(by left; (try by apply: Or31);(try by apply: Or32); apply: Or33);
+        right; (try by left); right.
+    have := s2Nu; have := vEs2.
+    by rewrite /valid_eval; move/valid_evalE : vEs2; rewrite mmE;
+          case; case=> ->;
+          case /or3P: (evalOr b (mk_move w i j)) => /eqP->.    
   rewrite -ltnNge => aLrs2. 
   apply: IH => //.
+  - by move/valid_evalE : vEs2; case; case => ->.
+  - by case/andP: Ums.
+  - rewrite /valid_sc (@get_max_cons (m, x) i j) //. 
+    apply: ltn_down_score scLrs2 => //.
+    - by have := evalOr b (mk_move w i j); case/or3P => /eqP->;
+        try (by apply: Or31); try (by apply: Or32); apply: Or33.
+    - by apply: get_max_range.
+    - by move: s2Nu; move/valid_evalE: vEs2; case; case=> -> //;
+      try(by left; (try by apply: Or31);(try by apply: Or32); apply: Or33);
+        right; (try by left); right.
+    - by move: scDu; move/valid_sc_range: Vsc; case; case=> -> //;
+      try(by left; (try by apply: Or31);(try by apply: Or32); apply: Or33);
+        right; (try by left); right.
+    have := s2Nu; have := vEs2.
+    by rewrite /valid_eval; move/valid_evalE : vEs2; rewrite mmE;
+          case; case=> ->;
+          case /or3P: (evalOr b (mk_move w i j)) => /eqP->.
   have betaE : (beta == draw) || (beta == win).
     by move: Vab; rewrite /valid_ab; case: eqP => // _ /andP[_ ->]; rewrite orbT.
   have alphaE : (alpha == loss) || (alpha == draw).
@@ -160,8 +363,43 @@ case: nltbP => [rs2Lb|/negP].
   by have [] := valid_evalE _ _ _ vEs2; case=> -> //=;
     case/orP : betaE => /eqP-> //.
 rewrite -leqNgt => bLrs2.
-case: nlebP => _; first by apply: IH.
-case: nlebP => [_|/negP]; first by apply: IH.
+case: nlebP => [Hd|/negP].
+  apply: IH => //; first by case/andP: Ums.
+  rewrite /valid_sc (@get_max_cons (m, x) i j) //.
+  apply: leq_down_score Hd => //.
+  - by have := evalOr b (mk_move w i j); case/or3P => /eqP->;
+      try (by apply: Or31); try (by apply: Or32); apply: Or33.
+  - by apply: get_max_range.
+  - by move: s2Nu; move/valid_evalE: vEs2; case; case=> -> //;
+    try(by left; (try by apply: Or31);(try by apply: Or32); apply: Or33);
+      right; (try by left); right.
+  - by move: scDu; move/valid_sc_range: Vsc; case; case=> -> //;
+    try(by left; (try by apply: Or31);(try by apply: Or32); apply: Or33);
+      right; (try by left); right.
+  have := s2Nu; have := vEs2.
+  by rewrite /valid_eval; move/valid_evalE : vEs2; rewrite mmE;
+        case; case=> ->;
+        case /or3P: (evalOr b (mk_move w i j)) => /eqP->.
+rewrite -ltnNge => scLrs2.
+case: nlebP => [_|/negP].
+  apply: IH => //.
+  - by move/valid_evalE : vEs2; case; case => ->.
+  - by case/andP: Ums.
+- rewrite /valid_sc (@get_max_cons (m, x) i j) //. 
+  apply: ltn_down_score scLrs2 => //.
+  - by have := evalOr b (mk_move w i j); case/or3P => /eqP->;
+      try (by apply: Or31); try (by apply: Or32); apply: Or33.
+  - by apply: get_max_range.
+  - by move: s2Nu; move/valid_evalE: vEs2; case; case=> -> //;
+    try(by left; (try by apply: Or31);(try by apply: Or32); apply: Or33);
+      right; (try by left); right.
+  - by move: scDu; move/valid_sc_range: Vsc; case; case=> -> //;
+    try(by left; (try by apply: Or31);(try by apply: Or32); apply: Or33);
+      right; (try by left); right.
+  have := s2Nu; have := vEs2.
+  by rewrite /valid_eval; move/valid_evalE : vEs2; rewrite mmE;
+          case; case=> ->;
+          case /or3P: (evalOr b (mk_move w i j)) => /eqP->.
 rewrite -ltnNge => aLrs2.
 case: (neqbP _ draw) => rs2Ed; last first.
   rewrite andFb.
@@ -170,7 +408,7 @@ case: (neqbP _ draw) => rs2Ed; last first.
       by have := rs2El; have [] := valid_evalE _ _ _ vEs2 => [] [] ->.
     case: neqbP => hsE.
       suff eD : DRAW <= eval w b <= DRAW.
-        rewrite andTb; case => dE _ <-.
+        rewrite andTb; case => dE _ <-; split; first by rewrite -dE.
         by apply: valid_has_table_valid_hput => //.
       have hsE1 : hs = lossdraw by apply: to_nat_inj.
       have {vEs2} := vEs2.
@@ -180,7 +418,7 @@ case: (neqbP _ draw) => rs2Ed; last first.
       apply/andP; split; last by case/andP: hsV1.
       by have := us2Le; rewrite s2E. 
     suff eD : down_score (rev_val s2) <= eval w b <= up_score (rev_val s2).
-      rewrite andTb; case => dE _ <-.
+      rewrite andTb; case => dE _ <-; split; first by rewrite -dE.
       by apply: valid_has_table_valid_hput.
     have {vEs2} := vEs2.
     rewrite s2E /valid_eval -[down_score _]/LOSS -[up_score _]/DRAW => vEs2.
@@ -188,7 +426,7 @@ case: (neqbP _ draw) => rs2Ed; last first.
     apply/andP; split; last by apply: leq_eval_win.
     by have := us2Le; rewrite s2E.  
   suff eD : down_score (rev_val s2) <= eval w b <= up_score (rev_val s2).
-    rewrite andFb; case => dE _ <-.
+    rewrite andFb; case => dE _ <-; split; first by rewrite -dE.
     by apply: valid_has_table_valid_hput.
   have s2El : s2 = loss.
     move: bLrs2 rs2Ed rs2El.
@@ -209,18 +447,34 @@ case: (boolP (is_nempty_move ms)) => ems.
   case: neqbP => hD.
     have hsE : hs = lossdraw by apply: to_nat_inj.
     suff eD : DRAW <= eval w b <= DRAW.
-      by case => dE _ <-; apply: valid_has_table_valid_hput.
+      case => dE _ <-; split; first by rewrite -dE.
+      by apply: valid_has_table_valid_hput.
     apply/andP; split; last first.
       by move: hsV; rewrite /valid_eval hsE; case/andP.
     by have := us2Le; rewrite s2E.
   suff eD : DRAW <= eval w b <= WIN.
-    by case => dE _ <-; apply: valid_has_table_valid_hput.
+    case => dE _ <-; split; first by rewrite -dE.
+    by apply: valid_has_table_valid_hput.
   apply/andP; split; last by apply: leq_eval_win.
   by have := us2Le; rewrite s2E.
 suff eD : DRAW <= eval w b <= DRAW.
-  rewrite s2E andFb; case => dE _ <-.
+  rewrite s2E andFb; case => dE _ <-; split; first by rewrite -dE.
   by apply: valid_has_table_valid_hput.
-admit.
+case: ms {IH}ems Ums Vms Vsc Vms1 => // ems Ums Vms Vsc Vms1.
+rewrite -get_max_nil (get_max_cons (m,x) i j) //.
+rewrite -{1}[DRAW]/(down_score (rev_val draw)) -{1}[DRAW]/(up_score (rev_val draw)).
+rewrite -s2E.
+apply: ltn_down_score scLrs2 => //.
+- by have /or3P[] := evalOr  b (mk_move w i j) => /eqP->; try (by apply: Or31);
+     try (by apply: Or32); apply: Or33.
+- by apply: get_max_range.
+- by rewrite s2E; left; apply: Or32.
+- by move: scDu; move/valid_sc_range : Vsc; case; case => -> //;
+     try(by left; (try by apply: Or31);(try by apply: Or32); apply: Or33);
+     right; (try by left); right.
+have := vEs2.
+rewrite /valid_eval s2E mmE.
+by have /or3P[] := evalOr  b (mk_move w i j) => /eqP->.
 Qed.
 
 Variables (wstate bstate : int) (beta : int) (lvisited : int) 
